$HK$ is a subgroup of $G$ $\implies$ $HK=KH$:  
- let $h\in H$ and $k\in K$, then $h^{-1}k^{-1}\in HK$. since $HK$ is a subgroup of $G$ and $(h^{-1}k^{-1})(kh)=1$, we have $kh \in HK$, that is $KH\sub HK$. since $k^{-1}h^{-1}\in HK$, then there exists $h_1\in H,k_1\in K$ such that $k^{-1}h^{-1}=h_1k_1$, then $1=(hk)(k^{-1}h^{-1})=(hk)(h_1k_1)$, we have $hk=k_1^{-1}h_1^{-1} \in KH$, that is $HK\sub KH$. in summary, we have $HK=KH$.

$HK=KH$ $\implies$ $HK$ is a subgroup of $G$:
- it is clear $1 \in HK$.
- let $h\in H$ and $k\in K$, then $hk\in HK$, then $k^{-1}h^{-1}\in KH=HK$, it is clear $k^{-1}h^{-1}$ is the inverse of $hk$. thus, we have every element of $HK$ has an inverse.
- let $h,h_1\in H$ and $k,k_1\in K$, then $hk,h_1k_1\in HK$. since $HK=KH$ and $kh_1\in KH$, then there exists $h_2\in H, k_2\in K$ such that $kh_1=h_2k_2$. then $(hk)(h_1k_1)=h(kh_1)k_1=h(h_2k_2)k_1\in HK$.