1. 
    - if $(u,w),(u',w')\in U\times W$, it is clear $(u,w)+(u',w')=(u+u',w+w')\in U\times W$.
    - if $(u,w),(u',w')\in U\times W$, then $(u,w)+(u',w')=(u+u',w+w')=(u',w')+(u,w)$.
    - since $0\in U$ and $0\in W$, then $(0,0)\in U\times W$. it is easy to verify that $(0,0)$ is the identity element.
    - if $(u,w)\in U\times W$, it is clear $(-u,-w)\in U\times W$. and since $(u,w)+(-u,-w)=(0,0)$, we have every element of $U\times W$ has an inverse.
    - if $(u,w),(u',w'),(u_1,w_1)\in U\times W$, then $((u,w)+(u',w'))+(u_1,w_1)=(u+u',w+w')+(u_1,w_1)=(u+u'+u_1,w+w'+w_1)$ and $(u,w)+((u',w')+(u_1,w_1))=(u,w)+(u'+u_1,w'+w_1)=(u+u'+u_1,w+w'+w_1)$, we have $((u,w)+(u',w'))+(u_1,w_1)=(u,w)+((u',w')+(u_1,w_1))$.

    thus, addition makes $U\times W$ into a commutative group.

    - if $(u,w)\in U\times W$ and $c\in F$, it is clear $c(u,w)=(cu,cw)\in U\times W$.
    - if $(u,w)\in U\times W$ and $1\in F$, then $1(u,w)=(1u,1w)=(u,w)$.
    - if $(u,w)\in U\times W$ and $a,b\in F$, then $(ab)(u,w)=(abu,abw)=a(bu,bw)=a(b(u,w))$.
    - if $(u,w)\in U\times W$ and $a,b\in F$, then $(a+b)(u,w)=((a+b)u,(a+b)w)=(au+bu,aw+bw)=(au,aw)+(bu,bw)=a(u,w)+b(u,w)$.
    - if $(u,w),(u',w')\in U\times W$ and $a\in F$, then $a((u,w)+(u',w'))=a(u+u',w+w')=(au+au',aw+aw')=(au,aw)+(au',aw')=a(u,w)+a(u',w')$.

    in summary, we have $U\times W$ is a vector space.
2. 
    - if $(u,w),(u',w')\in U\times W$, then $T((u,w)+(u',w'))=u+u'+w+w'=T((u,w))+T((u',w'))$.
    - if $(u,w)\in U\times W$ and $c\in F$, then $T(c(u,w))=cu+cw=c(u+w)=cT((u,w))$.

    thus, we have $T$ is a linear transformation.
3. it is clear $\text{im } T=U+W$.  
let $B=(v_1,\dots,v_n)$ be a basis of $U\cap W$, we claim $B'=((v_1,-v_1),\dots,(v_n,-v_n))$ is a basis of $\ker T$.
    - if $a_1(v_1,-v_1)+\dots+a_n(v_n,-v_n)=0$, that is $(a_1 v_1+\dots+a_n v_n,-a_1 v_1-\dots-a_n v_n)=0$. since $B$ is a basis, we have $a_1=\dots=a_n=0$. thus, $(v_1,-v_1),\dots,(v_n,-v_n)$ are independent. 
    - if $v\in \ker T$, then there exists $u\in U,w\in W$ such that $v=(u,w)$ and $T(v)=u+w=0$, we have $w=-u$, it is clear $u,w\in U\cap W$. thus, $\ker T\sub \text{Span } B'$.
    - if $v\in \text{Span } B'$, it is easy to verify $T(v)=0$. thus, we have $\text{Span } B'\sub \ker T$.

    since $\text{Span } B'= \ker T$, we have $\dim (\ker T)=\dim (U\cap W)$, then $\dim T=\dim (\ker T)+\dim (\text{im } T)=\dim (U\cap W)+\dim (U+W)=\dim U +\dim W$.
