let
$A=\begin{bmatrix}
   a_{1,1} & a_{1,2}   \\
   a_{2,1} & a_{2,2} 
\end{bmatrix},
B=\begin{bmatrix}
   b_{1,1} & b_{1,2}   \\
   b_{2,1} & b_{2,2} 
\end{bmatrix}$
then
$T(e_{1,1})=Ae_{1,1}B=
\begin{bmatrix}
   a_{1,1}   \\
   a_{2,1} 
\end{bmatrix}
\begin{bmatrix}
   b_{1,1} & b_{1,2}   \\ 
\end{bmatrix}$
$T(e_{1,2})=Ae_{1,2}B=
\begin{bmatrix}
   a_{1,1}   \\
   a_{2,1} 
\end{bmatrix}
\begin{bmatrix}
   b_{2,1} & b_{2,2}   \\ 
\end{bmatrix}$
$T(e_{2,1})=Ae_{2,1}B=
\begin{bmatrix}
   a_{1,2}   \\
   a_{2,2} 
\end{bmatrix}
\begin{bmatrix}
   b_{1,1} & b_{1,2}   \\ 
\end{bmatrix}$
$T(e_{2,2})=Ae_{2,2}B=
\begin{bmatrix}
   a_{1,2}   \\
   a_{2,2} 
\end{bmatrix}
\begin{bmatrix}
   b_{2,1} & b_{2,2}   \\ 
\end{bmatrix}$
  
then $T((e_{1,1},e_{1,2},e_{2,1},e_{2,2}))=(T(e_{1,1}),T(e_{1,2}),T(e_{2,1}),T(e_{2,2}))=$
$(e_{1,1},e_{1,2},e_{2,1},e_{2,2})
\begin{bmatrix}
   a_{1,1}b_{1,1} & a_{1,1}b_{2,1} & a_{1,2}b_{1,1} & a_{1,2}b_{2,1}  \\
   a_{1,1}b_{1,2} & a_{1,1}b_{2,2} & a_{1,2}b_{1,2} & a_{1,2}b_{2,2}   \\ 
   a_{2,1}b_{1,1} & a_{2,1}b_{2,1} & a_{2,2}b_{1,1} & a_{2,2}b_{2,1}    \\
   a_{2,1}b_{1,2} & a_{2,1}b_{2,2} & a_{2,2}b_{1,2} & a_{2,2}b_{2,2}   
\end{bmatrix}$
we have the matrix of the operator $T$ is
$\begin{bmatrix}
   a_{1,1}b_{1,1} & a_{1,1}b_{2,1} & a_{1,2}b_{1,1} & a_{1,2}b_{2,1}  \\
   a_{1,1}b_{1,2} & a_{1,1}b_{2,2} & a_{1,2}b_{1,2} & a_{1,2}b_{2,2}   \\ 
   a_{2,1}b_{1,1} & a_{2,1}b_{2,1} & a_{2,2}b_{1,1} & a_{2,2}b_{2,1}    \\
   a_{2,1}b_{1,2} & a_{2,1}b_{2,2} & a_{2,2}b_{1,2} & a_{2,2}b_{2,2}   
\end{bmatrix}$