1. since $T(v-T(v))=T(v)-T^2(v)=T(v)-v=-1(v-T(v))$, we have if $v-T(v)\not=0$, then $v-T(v)$ is an eigenvector with eigenvalue $-1$. similarly, if $v+T(v)\not=0$, then $v+T(v)$ is an eigenvector with eigenvalue $1$. thus, we have $v-T(v)\in V^{(-1)}$ and $v+T(v)\in V^{(1)}$, then $2v=(v-T(v))+(v+T(v))\in V^{(-1)}+V^{(1)}$, then $V^{(-1)}+V^{(1)}=V$.  
suppose $V^{(-1)}\cap V^{(1)}\not=\{0\}$, then there exists $v_1\not=0$ such that $v_1\in V^{(-1)}\cap V^{(1)}$, then $T(v_1)=v_1$ and $T(v_1)=-v_1$, we have $v_1=0$, it is impossible. thus, we must have $V^{(-1)}\cap V^{(1)}=\{0\}$.  
since $V^{(-1)}\cap V^{(1)}=\{0\}$ and $V^{(-1)}+V^{(1)}=V$, we have $V=V^{(-1)}\oplus V^{(1)}$.
2. let $v\in V$, since $T(v+T(v)+T^2(v)+T^3(v))=T(v)+T^2(v)+T^3(v)+v$, we have if $v+T(v)+T^2(v)+T^3(v)\not=0$, then $v+T(v)+T^2(v)+T^3(v)$ is an eigenvector with eigenvalue $1$. similarly, if $v-T(v)+T^2(v)-T^3(v),v+iT(v)-T^2(v)-iT^3(v),v-iT(v)-T^2(v)+iT^3(v)\not=0$, then $v-T(v)+T^2(v)-T^3(v),v+iT(v)-T^2(v)-iT^3(v),v-iT(v)-T^2(v)+iT^3(v)$ are eigenvectors with eigenvalues $1,i,-i$. thus, we have $v+T(v)+T^2(v)+T^3(v)\in V^{(1)},v-T(v)+T^2(v)-T^3(v)\in V^{(-1)},v+iT(v)-T^2(v)-iT^3(v)\in V^{(i)},v-iT(v)-T^2(v)+iT^3\in V^{(-i)}$, then $4v=(v+T(v)+T^2(v)+T^3(v))+(v-T(v)+T^2(v)-T^3(v))+(v+iT(v)-T^2(v)-iT^3(v))+(v-iT(v)-T^2(v)+iT^3(v))\in V^{(1)}+V^{(-1)}+V^{(i)}+V^{(-i)}$, then $V^{(1)}+V^{(-1)}+V^{(i)}+V^{(-i)}=V$.  
let $v_1\in V^{(1)},v_2\in V^{(-1)},v_3\in V^{(i)},v_4\in V^{(-i)}$, if $v_1+v_2+v_3+v_4=0$, then $T(v_1+v_2+v_3+v_4)=0,T^2(v_1+v_2+v_3+v_4)=0,T^3(v_1+v_2+v_3+v_4)=0$, we have
$(v_1,v_2,v_3,v_4)\begin{bmatrix}
   1 & 1  & 1 & 1  \\
   1 & -1 & 1 & -1 \\
   1 & i & -1 & -i  \\
   1 & -i & -1 & i \\
\end{bmatrix}=0$
then $v_1=v_2=v_3=v_4=0$. thus, $V^{(1)},V^{(-1)},V^{(i)},V^{(-i)}$ are independent.  
since $V^{(1)},V^{(-1)},V^{(i)},V^{(-i)}$ are independent and $V^{(1)}+V^{(-1)}+V^{(i)}+V^{(-i)}=V$, we have $V=V^{(1)}\oplus V^{(-1)}\oplus V^{(i)}\oplus V^{(-i)}$.