1. since 
$\begin{bmatrix}
   a & b \\
   c & d 
\end{bmatrix}
\begin{bmatrix}
   x_1  \\
   s\cdot x_1 
\end{bmatrix}=
\begin{bmatrix}
   y_1  \\
   s \cdot y_1 
\end{bmatrix}$
we have
$\begin{cases}
   ax_1+bs \cdot x_1=y_1 \\
   cx_1+ds \cdot x_1=s \cdot y_1
\end{cases}$
then $bs^2+(a-d)s-c=0$.
2. since $bs^2+(a-d)s-c=0$, we have $s=\frac{d-a-\sqrt{(a-d)^2+4bc}}{2b}$ or $s=\frac{d-a+\sqrt{(a-d)^2+4bc}}{2b}$, note that $\sqrt{(a-d)^2+4bc}>|d-a|$, it is clear there is an eigenvector in the first quadrant and also one in the second quadrant.