let $B=(v_0,\dots,v_n)$, then $T(B)=(T(v_0),\dots,T(v_n))=$
$B\begin{bmatrix}
   0 & 0 & \dots & 0 & 0 & a_0\\
   1 & 0 & \dots & 0 & 0 & a_1\\
   0 & 1 & \dots & 0 & 0 & a_2\\
   0 & 0 & \dots & 0 & 0 & a_3\\
   \vdots & \vdots & \ddots & \vdots & \vdots & \vdots \\
   0 & 0 & \dots & 0 & 0 & a_{n-2}\\
   0 & 0 & \dots & 1 & 0 & a_{n-1}\\
   0 & 0 & \dots & 0 & 1 & a_n\\
\end{bmatrix}$
let $A$ be the matrix of $T$, then
$A=\begin{bmatrix}
   0 & 0 & \dots & 0 & 0 & a_0\\
   1 & 0 & \dots & 0 & 0 & a_1\\
   0 & 1 & \dots & 0 & 0 & a_2\\
   0 & 0 & \dots & 0 & 0 & a_3\\
   \vdots & \vdots & \ddots & \vdots & \vdots & \vdots \\
   0 & 0 & \dots & 0 & 0 & a_{n-2}\\
   0 & 0 & \dots & 1 & 0 & a_{n-1}\\
   0 & 0 & \dots & 0 & 1 & a_n\\
\end{bmatrix}$
for $k=0,\dots,n$, let
$B_k=\begin{bmatrix}
   0 & 0 & \dots & 0 & 0 & a_{n-k}\\
   1 & 0 & \dots & 0 & 0 & a_{n-k+1}\\
   0 & 1 & \dots & 0 & 0 & a_{n-k+2}\\
   0 & 0 & \dots & 0 & 0 & a_{n-k+3}\\
   \vdots & \vdots & \ddots & \vdots & \vdots & \vdots \\
   0 & 0 & \dots & 0 & 1 & a_n\\
\end{bmatrix}$
it is clear $A=B_n$, and let $p_{k}(t)=\det (t I-B_k)$, then we have $p_{n}(t)=\det(t I-A)$. it is easy to verify that $p_{k}(t)=t\cdot p_{k-1}(t)-a_{n-k}$, we have $p_{n}(t)=t^{n+1}-a_{n}t^n-a_{n-1}t^{n-1}-\dots-a_0$.